Protocols/RB/Liveness_tla.v
@@ -1,0 +1,41 @@
+From Coq Require Import List Bool Lia PeanoNat ListSet Permutation RelationClasses.
+From Coq Require ssrbool ssreflect.
+Import (coercions) ssrbool.
+Import ssreflect.SsrSyntax.
+From ABCProtocol.Protocols.RB Require Export Liveness.
+
+From ABCProtocol.Properties Require Export Liveness_tla.
+
+Module RBLiveness2 (A : NetAddr) (R : RBTag) (V : Signable) (VBFT : ValueBFT A R V)
+  (BTh : ClassicByzThreshold A) (BSett : RestrictedByzSetting A BTh).
+
+Import A R V VBFT BTh BSett.
+Import ssrbool. (* anyway *)
+
+Module Export RBLive := RBLiveness A R V VBFT BTh BSett.
+Include Liveness A M BTh BSett P PSOp RBP Ns RBAdv RBN.
+
+Lemma global_liveness_in_tla src r v :
+  ⌜ init ⌝ ∧ □ ⟨ next ⟩ ∧ fairness ⊢
+  ⌜ some_receives src r v ⌝ ~~> ⌜ all_receives src r v ⌝.
+Proof.
+  tla_apply (leads_to_trans _ (⌜ round_2_start src r v ⌝)).
+  tla_split.
+  - apply leads_to_by_eventual_delivery.
+    intros w H_w_reachable H. pose proof (round_1_pkts H_w_reachable H) as (nonbyz_senders & pkts & Hround1).
+    hnf in Hround1. pose proof Hround1 as HH. destruct_and? Hround1.
+    exists pkts. split_and?; auto. 
+    intros w0 l0 Htrace0 -> Hincl.
+    eapply round_2_start_suffcond; eauto.
+    eapply round_1_end_suffcond; eauto. 
+  - apply leads_to_by_eventual_delivery.
+    intros w H_w_reachable H. pose proof (round_2_pkts H_w_reachable H) as (pkts & Hround2).
+    hnf in Hround2. pose proof Hround2 as HH. destruct_and? Hround2.
+    exists pkts. split_and?; auto. 
+    intros w0 l0 Htrace0 -> Hincl.
+    eapply all_receives_suffcond; eauto.
+    eapply round_2_end_suffcond; eauto.
+Qed.
+
+End RBLiveness2.
+
